# Prática 6 - Ex 3

### 1) ( λ x . 2 * x + 1) 3

 ( λ x . 2 * x + 1) 3

2 * 3 + 1

6 + 1 → 7

### 2) ( λ xy . x - y) 5 7

( λ y . 5 - y ) 7

5 - 7 → -2

### 3) ( λ yx . x - y) 5 7

( λ x . x - 5 ) 7

7 - 5 → 2

### 4) ( λ xy . x - y) ( λ z . z/2)

( λ y . ( λ z . z/2) - y)

### 5) ( λ xy . x - y) ( ( λ z . z/2) 6) 1

( λ xy . x - y) (6/2) 1

( λ xy . x - y) 3 1

( λ y . 3 - y ) 1

3 - 1 → 2

### 6) ( λ x. λ y . - x y) 9 4

 ( λ y . - 9 y) 4

(- 9 4)

9 - 4 → 5

### 7) ( λ x . xx ) ( λ y . y)

( λ y . y ) ( λ y . y )

( λ y . y )
